coq/LLVMGen/Correctness_AExpr.v
@@ -1,77 +1,10 @@
-Require Import Coq.Arith.Arith.
-Require Import Psatz.
-
-Require Import Coq.Strings.String.
-
-Open Scope string_scope.
-Open Scope char_scope.
-
-Require Import Coq.Lists.List.
-
-Require Import Coq.Numbers.BinNums. (* for Z scope *)
-Require Import Coq.ZArith.BinInt.
-
-Require Import Helix.FSigmaHCOL.FSigmaHCOL.
-Require Import Helix.FSigmaHCOL.Int64asNT.
-Require Import Helix.FSigmaHCOL.Float64asCT.
-Require Import Helix.DSigmaHCOL.DSigmaHCOLITree.
-Require Import Helix.LLVMGen.Compiler.
-Require Import Helix.LLVMGen.Data.
-Require Import Helix.LLVMGen.Utils.
-Require Import Helix.LLVMGen.tmp_aux_Vellvm.
-Require Import Helix.Util.OptionSetoid.
-Require Import Helix.Util.ErrorSetoid.
-Require Import Helix.Util.ListUtil.
-Require Import Helix.Tactics.HelixTactics.
-
-Require Import ExtLib.Structures.Monads.
-Require Import ExtLib.Data.Map.FMapAList.
-
-Require Import Vellvm.Tactics.
-Require Import Vellvm.Util.
-Require Import Vellvm.LLVMEvents.
-Require Import Vellvm.DynamicTypes.
-Require Import Vellvm.Denotation.
-Require Import Vellvm.Handlers.Handlers.
-Require Import Vellvm.TopLevel.
-Require Import Vellvm.LLVMAst.
-Require Import Vellvm.CFG.
-Require Import Vellvm.InterpreterMCFG.
-Require Import Vellvm.InterpreterCFG.
-Require Import Vellvm.TopLevelRefinements.
-Require Import Vellvm.TypToDtyp.
-Require Import Vellvm.LLVMEvents.
-Require Import Vellvm.Denotation_Theory.
-Require Import Vellvm.InstrLemmas.
-
-Require Import Ceres.Ceres.
-
-Require Import ITree.Interp.TranslateFacts.
-Require Import ITree.Basics.CategoryFacts.
-Require Import ITree.Events.State.
-Require Import ITree.Events.StateFacts.
-Require Import ITree.ITree.
-Require Import ITree.Eq.Eq.
-Require Import ITree.Basics.Basics.
-Require Import ITree.Interp.InterpFacts.
-
-Require Import Flocq.IEEE754.Bits.
-
-Require Import MathClasses.interfaces.canonical_names.
-Require Import MathClasses.misc.decision.
-
+Require Import Helix.LLVMGen.Correctness_Prelude.
 Require Import Helix.LLVMGen.Correctness_Invariants.
 Require Import Helix.LLVMGen.Correctness_NExpr.
 Require Import Helix.LLVMGen.Correctness_MExpr.
 
 Set Implicit Arguments.
 Set Strict Implicit.
-
-Import MDSHCOLOnFloat64.
-Import D.
-Import ListNotations.
-Import MonadNotation.
-Local Open Scope monad_scope.
 
 Typeclasses Opaque equiv.
 Remove Hints
@@ -724,7 +657,8 @@ Section AExpr.
 
       epose proof (AEXPR l2 _) as [EUTT EVAL'].
       rewrite denote_code_singleton.
-
+      (* YZ TODO: should not have made assoc opaque *)
+      Transparent assoc.
       rewrite denote_instr_intrinsic; cbn.
       2,3:reflexivity.
       4: {
@@ -1358,31 +1292,37 @@ Section AExpr.
         set (alist_add (Traversal.endo r) (dvalue_to_uvalue (double_cmp (Traversal.endo FOlt) b' b'')) l'') as l'''.
         pose proof denote_conversion_concrete Uitofp (DTYPE_I 1) DTYPE_Double (EXP_Ident (ID_Local (Traversal.endo r))) g'' l''' memV'' x (dvalue_to_uvalue (double_cmp (Traversal.endo FOlt) b' b'')).
         rewrite typ_to_dtyp_equation.
-        rewrite H.
-        reflexivity.
-        rewrite uvalue_to_dvalue_of_dvalue_to_uvalue. reflexivity.
         cbn.
-        unfold Traversal.endo.
-        unfold Traversal.Endo_id.
-        match_rewrite.
-        reflexivity.
+        (* YZ: Sorry I broke this one but this is too ugly to debug, we'll have to redo the proof anyway.
+           The goal is to have Vellvm side automation in the style of norm for this.
+         *)
+        admit.
 
-        cbn.
-        rewrite translate_trigger.
-        rewrite translate_trigger.
-        rewrite lookup_E_to_exp_E_Local.
-        rewrite subevent_subevent.
-        rewrite exp_E_to_instr_E_Local.
-        rewrite subevent_subevent.
-        rewrite interp_cfg_to_L3_LR.
-        cbn.
+        (* rewrite H. *)
+        (* reflexivity. *)
+        (* rewrite uvalue_to_dvalue_of_dvalue_to_uvalue. reflexivity. *)
+        (* cbn. *)
+        (* unfold Traversal.endo. *)
+        (* unfold Traversal.Endo_id. *)
+        (* match_rewrite. *)
+        (* reflexivity. *)
 
-        reflexivity.
+        (* cbn. *)
+        (* rewrite translate_trigger. *)
+        (* rewrite translate_trigger. *)
+        (* rewrite lookup_E_to_exp_E_Local. *)
+        (* rewrite subevent_subevent. *)
+        (* rewrite exp_E_to_instr_E_Local. *)
+        (* rewrite subevent_subevent. *)
+        (* rewrite interp_cfg_to_L3_LR. *)
+        (* cbn. *)
 
-        (* Lookup *)
-        unfold Traversal.endo, Traversal.Endo_id in *.
-        subst l'''.
-        apply In_add_eq.
+        (* reflexivity. *)
+
+        (* (* Lookup *) *)
+        (* unfold Traversal.endo, Traversal.Endo_id in *. *)
+        (* subst l'''. *)
+        (* apply In_add_eq. *)
       }
 
       norm_v.
@@ -1393,11 +1333,11 @@ Section AExpr.
         eapply state_invariant_incVoid; eauto.
         repeat (eapply state_invariant_add_fresh; eauto).
       + split; split; intuition.
-          * cbn. repeat norm_v. cbn. norm_v.
+          * cbn. repeat norm_v. cbn.
             reflexivity.
             cbn.
             apply H.
-            rewrite <- CMP_H.
+            rewrite CMP_H.
 
             apply In_add_eq.
           * cbn.
@@ -1411,8 +1351,6 @@ Section AExpr.
             assert (l' ⊑ l'') as L'L'' by auto.
             rewrite L1L', L'L''.
 
-            unfold Traversal.endo, Traversal.Endo_id.
-            rewrite CMP_V.
             cbn.
 
             assert (l'' ⊑ (alist_add r (UVALUE_I1 cmp_res) l'')) as TRANS.
